denotation for separation logic formula. - things are still in flux TODOs: - reflect with automation, - write a prover for separation logic.

src/SepTheory.v
@@ -13,37 +13,103 @@ End SepLog.
 Module Make (M : SepLog).
   Import M.
 
-  Definition smem := list (addr * byte).
+  Definition mem := addr -> byte.
+
+  Definition smem := addr -> option byte.
+
+  Definition satisfies (s : smem) (m : mem) : Prop :=
+    forall p, match s p with
+                | None => True
+                | Some x => m p = x
+              end.
 
   Definition hprop : Type := smem -> Prop.
 
-  Fixpoint smem_lookup (p : addr) (m : smem) : option byte :=
-    match m with
-      | nil => None
-      | a :: b => if addr_dec (fst a) p then Some (snd a) else smem_lookup p b
-    end.
+  Definition disjoint (m1 m2 : smem) : Prop :=
+    forall p, m1 p = None \/ m2 p = None.
 
-  Fixpoint disjoint (m1 m2 : smem) : Prop :=
-    match m1 with
-      | nil => True
-      | a :: b => smem_lookup (fst a) m2 = None /\ disjoint b m2
-    end.
+  Definition join (m1 m2 : smem) : smem := 
+    fun p => match m1 p with
+               | None => m2 p
+               | v => v
+             end.
 
-  Definition join (m1 m2 : smem) : smem := m1 ++ m2.
+  Definition smem_eq (a b : smem) : Prop := forall p, a p = b p.
+  Infix "===" := smem_eq (at level 50).
 
   Definition split (m ml mr : smem) : Prop :=
-    disjoint ml mr /\
-    forall a, smem_lookup a m = smem_lookup a (join ml mr).
+    disjoint ml mr /\ m === join ml mr.
 
   Definition semp : hprop := 
-    fun h => h = nil.
+    fun h => forall p, h p = None.
 
   Definition ptsTo (a : addr) (b : byte) : hprop :=
-    fun h => h = (a,b) :: nil.
+    fun h => h a = Some b /\ forall p, p <> a -> h p = None.
+
+  Definition star (P Q : hprop) : hprop :=
+    fun h => exists hl, exists hr, split h hl hr /\ P hl /\ Q hr.
 
   Definition ex (T : Type) (p : T -> hprop) : hprop :=
     fun v => exists x, p x v.
 
+  Definition himp (P Q : hprop) : Prop :=
+    forall h, P h -> Q h.
+
+  Infix "==>" := (himp) (at level 50).
+
+
+  
+
+  Require Import Classes.RelationClasses.
+  Global Instance Refl_smem : Reflexive smem_eq.
+  Proof.
+    red. firstorder.
+  Qed.
+
+  Global Instance Sym_smem : Symmetric smem_eq.
+  Proof.
+    red. firstorder.
+  Qed.
+  
+  Global Instance Trans_smem : Transitive smem_eq.
+  Proof.
+    red. unfold smem_eq. firstorder. rewrite H. auto.
+  Qed.
+
+
+  
+  Lemma disjoint_join : forall a b, disjoint a b -> join a b === join b a.
+  Proof.
+    intros. red. intros. unfold join, disjoint in *. specialize (H p). destruct (a p); destruct (b p); try congruence.
+    exfalso; firstorder; congruence.
+  Qed.
+    
+  Lemma disjoint_comm : forall ml mr, disjoint ml mr -> disjoint mr ml.
+  Proof.
+    firstorder.
+  Qed.
+
+  Lemma split_comm : forall m ml mr, split m ml mr -> split m mr ml.
+  Proof.
+    unfold split. intros. destruct H. apply disjoint_comm in H. split; auto. rewrite disjoint_join; auto.
+  Qed.
+
+  Theorem star_comm : forall P Q, star P Q ==> star Q P.
+  Proof.
+    intros. unfold himp, star. firstorder. apply disjoint_comm in H. 
+    do 3 eexists. unfold split. 2: split; eassumption. rewrite disjoint_join; auto.
+  Qed.
+
+  Theorem star_assoc : forall P Q R, star P (star Q R) ==> star (star P Q) R.
+  Proof.
+  (*
+    unfold himp, star. intros.
+    do 2 destruct H. intuition. destruct H2. destruct H1. intuition.
+    do 2 eexists. split. 2: split; try eassumption. 2: do 2 eexists. 2: split. 3: split; eassumption.
+    unfold split. 
+  *)
+  Admitted.
+   
 
   (** separation logic theory **)
   (** I need to denote this in terms of PropX **)
