src/SepExpr.v
@@ -1,63 +1,59 @@
 Require Import List.
 Require Import Expr.
 Require Import SepTheory PropX.
+Require Import IL.
 
 Set Implicit Arguments.
 
 Module SepExpr (B : SepLog).
   Module L := Make B.  
 
-Section env.
+  Section env.
 
-  Variable types : list type.
-  Variable funcs : functions types.
+    Variable types : list type.
+    Variable funcs : functions types.
 
-  Variable pcType : tvar types.    
-  Variable stateType : tvar types.
+    Variable pcType : tvar types.    
+    Variable stateType : tvar types.
+    Variable stateMem : tvarD stateType -> L.mem.
 
-  Record ssignature := {
-    SDomain : list (tvar types) ;
-    SDenotation : functionTypeD (map (@tvarD types) SDomain) (L.smem -> PropX (tvarD pcType) (tvarD stateType))
-  }.
-  Variable sfuncs : list ssignature.
+    Record ssignature := {
+      SDomain : list (tvar types) ;
+      SDenotation : functionTypeD (map (@tvarD types) SDomain) (L.smem -> PropX (tvarD pcType) (tvarD stateType))
+    }.
+    Variable sfuncs : list ssignature.
 
-  Inductive sexpr : variables types -> Type :=
-  | Inj : forall vars, expr funcs vars None -> sexpr vars
-  | Star : forall vars, sexpr vars -> sexpr vars -> sexpr vars
-  | Exists : forall vars t, sexpr (t :: vars) -> sexpr vars
-  | Cptr : forall vars, expr funcs vars pcType -> sexpr (stateType :: vars) -> sexpr vars
-  | Func : forall vars (f : fin sfuncs), 
-    hlist (expr funcs vars) (SDomain (get sfuncs f)) -> sexpr vars
-  | Const : forall vars, 
-    PropX (tvarD pcType) (tvarD stateType) -> sexpr vars
-    (** PtsTo should be derived, that way we can handle different sizes easily **)
-  .
+    Inductive sexpr : variables types -> Type :=
+    | Inj : forall vars, expr funcs vars None -> sexpr vars
+    | Star : forall vars, sexpr vars -> sexpr vars -> sexpr vars
+    | Exists : forall vars t, sexpr (t :: vars) -> sexpr vars
+    | Cptr : forall vars, expr funcs vars pcType -> sexpr (stateType :: vars) -> sexpr vars
+    | Func : forall vars (f : fin sfuncs), 
+      hlist (expr funcs vars) (SDomain (get sfuncs f)) -> sexpr vars
+    | Const : forall vars, 
+      PropX (tvarD pcType) (tvarD stateType) -> sexpr vars
+    (** PtsTo should be derived, that way we can handle different sizes easily, 
+     ** baking it in allows us to derive <> facts from points to 
+     **)
+      .
 
-  Fixpoint sexprD (vars : variables types) (s : sexpr vars)
-    : hlist (@tvarD types)  vars -> L.smem -> PropX (tvarD pcType) (tvarD stateType) :=
-    match s in sexpr vars return hlist (@tvarD types) vars -> L.smem -> PropX (tvarD pcType) (tvarD stateType) with
-      | Inj _ p => fun g _ => PropX.Inj (exprD g p)
-      | Exists _ t b => fun g m => PropX.Exists (fun x : tvarD t => sexprD b (HCons x g) m)
-      | Func _ f b => fun g =>
-        applyD (exprD g) b _ (SDenotation (get sfuncs f))
-      | Const _ p => fun _ _ => p
-      | Star _ l r => fun g m => 
-        PropX.Exists (fun ml : L.smem => PropX.Exists (fun mr : L.smem => 
-          PropX.And (PropX.Inj (L.split m ml mr)) (And (sexprD l g ml) (sexprD l g mr))))
-      | Cptr _ p t => fun g m =>
-        (** TODO: I need to connect m to x **)
-        PropX.Cptr (exprD g p) 
-          (fun x : tvarD stateType => PropX.Exists (fun m => PropX.And (PropX.Inj True) (sexprD t (HCons x g) m)))
-    end.
+    Fixpoint sexprD (vars : variables types) (s : sexpr vars)
+      : hlist (@tvarD types)  vars -> L.smem -> PropX (tvarD pcType) (tvarD stateType) :=
+      match s in sexpr vars return hlist (@tvarD types) vars -> L.smem -> PropX (tvarD pcType) (tvarD stateType) with
+        | Inj _ p => fun g _ => PropX.Inj (exprD g p)
+        | Exists _ t b => fun g m => PropX.Exists (fun x : tvarD t => sexprD b (HCons x g) m)
+        | Func _ f b => fun g =>
+          applyD (exprD g) b _ (SDenotation (get sfuncs f))
+        | Const _ p => fun _ _ => p
+        | Star _ l r => fun g m => 
+          PropX.Exists (fun ml : L.smem => PropX.Exists (fun mr : L.smem => 
+            PropX.And (PropX.Inj (L.split m ml mr)) (And (sexprD l g ml) (sexprD l g mr))))
+        | Cptr _ p t => fun g m =>
+          PropX.Cptr (exprD g p) 
+          (fun x : tvarD stateType => PropX.Exists (fun m => 
+            PropX.And (PropX.Inj (L.satisfies m (stateMem x))) (sexprD t (HCons x g) m)))
+      end.
 
-End env.
-
-
-
-
+  End env.
 
 End SepExpr.
-
-
-
-
